LTS.thy
@@ -27,7 +27,7 @@ primrec LTS_is_reachable :: "('q, 'a) LTS \<Rightarrow> 'q \<Rightarrow> 'a list
       (\<exists>q'' \<sigma>. a \<in> \<sigma> \<and> (q, \<sigma>, q'') \<in> \<Delta> \<and> LTS_is_reachable \<Delta> q'' w q')"
 
 
-lemma DeltLTSlemma:"LTS_is_reachable Δ q x y \<Longrightarrow>LTS_is_reachable {(f a, b, f c)| a b c. (a,b,c)\<in> Δ } (f q) x (f y)"
+lemma DeltLTSlemma:"LTS_is_reachable \<Delta> q x y \<Longrightarrow>LTS_is_reachable {(f a, b, f c)| a b c. (a,b,c)\<in> \<Delta> } (f q) x (f y)"
   apply(induct x arbitrary:q)
    apply simp
   apply simp
@@ -77,40 +77,40 @@ inductive_cases LTS_Epi1_cases[elim!]:"LTS_is_reachable \<Delta> q l q"
 
 
 
-lemma DeltLTSlemma1:"LTS_is_reachable Δ q al y \<Longrightarrow>LTS_is_reachable {(f u, v, f w)| u v w. (u,v,w)\<in> Δ } (f q) al (f y)"
+lemma DeltLTSlemma1:"LTS_is_reachable \<Delta> q al y \<Longrightarrow>LTS_is_reachable {(f u, v, f w)| u v w. (u,v,w)\<in> \<Delta> } (f q) al (f y)"
   proof (induction rule: LTS_is_reachable.induct)
-    case (LTS_Empty Δ q)
+    case (LTS_Empty \<Delta> q)
     then show ?case 
       by (simp add: LTS_is_reachable.LTS_Empty)
   next
-    case (LTS_Step a q Δ w q')
+    case (LTS_Step a q \<Delta> w q')
     then show ?case 
       by (smt (verit, best) CollectI LTS_is_reachable.LTS_Step)
   next
-    case (LTS_Epi q Δ q')
+    case (LTS_Epi q \<Delta> q')
     then show ?case 
       by (smt (verit, ccfv_threshold) CollectI LTS_is_reachable.LTS_Epi)
   next
-    case (LTS_Epi1 q Δ l q')
+    case (LTS_Epi1 q \<Delta> l q')
     then show ?case 
       by (metis (mono_tags, lifting) CollectI LTS_is_reachable.LTS_Epi1)
   qed
 
 lemma subLTSlemma:"LTS_is_reachable l1 q x y \<Longrightarrow> LTS_is_reachable (l1 \<union> l2) q x y"
   proof (induction rule: LTS_is_reachable.induct)
-    case (LTS_Empty Δ q)
+    case (LTS_Empty \<Delta> q)
     then show ?case 
       by (simp add: LTS_is_reachable.LTS_Empty)
   next
-    case (LTS_Step a q Δ w q')
+    case (LTS_Step a q \<Delta> w q')
     then show ?case 
       by (meson LTS_is_reachable.LTS_Step UnI1)
   next
-    case (LTS_Epi q Δ q')
+    case (LTS_Epi q \<Delta> q')
     then show ?case 
       by (meson LTS_is_reachable.LTS_Epi Un_iff)
   next
-    case (LTS_Epi1 q Δ l q')
+    case (LTS_Epi1 q \<Delta> l q')
     then show ?case 
       by (meson LTS_is_reachable.LTS_Epi1 UnI1)
   qed
@@ -120,19 +120,19 @@ lemma subLTSlemma:"LTS_is_reachable l1 q x y \<Longrightarrow> LTS_is_reachable 
 
 lemma joinLTSlemma:"LTS_is_reachable l1 q a y \<Longrightarrow> LTS_is_reachable l1 y b z \<Longrightarrow> LTS_is_reachable l1 q (a@b) z"
   proof (induction rule: LTS_is_reachable.induct)
-    case (LTS_Empty Δ q)
+    case (LTS_Empty \<Delta> q)
     then show ?case 
       by simp
   next
-    case (LTS_Step a q Δ w q')
+    case (LTS_Step a q \<Delta> w q')
     then show ?case 
       by (metis LTS_is_reachable.LTS_Step append_Cons)
   next
-    case (LTS_Epi q Δ q')
+    case (LTS_Epi q \<Delta> q')
     then show ?case 
       by (meson LTS_Epi1)
   next
-    case (LTS_Epi1 q Δ l q')
+    case (LTS_Epi1 q \<Delta> l q')
     then show ?case 
       by (meson LTS_is_reachable.LTS_Epi1)
   qed
