test.thy
@@ -1,5 +1,0 @@
-theory test 
-  imports Main
-begin
-fun a :: "'a \<Rightarrow> 'b" where
-end
